squashed saw-core-coq changes from wip-heapster (...)
- GaloisInc/saw-core@59e6108 move prod destructing to after prove_refinement_eauto
- GaloisInc/saw-core@6028a21 remove bitvector type synonym from Prelude (needs latest heapster-saw)
- GaloisInc/saw-core@bf6cd78 remove EqP, replace with Eq (needs latest heapster-saw)
- GaloisInc/saw-core@a2d632c composeM is no longer skipped by the Coq translator
- GaloisInc/saw-core@9fa8e4f add IRT_BVVec, add gen_at_BVVec for IRT isomorphism
- GaloisInc/saw-core@7e098d5 prove foldIRT/unfoldIRT isomorphism
- GaloisInc/saw-core@0e53c87 use `match`es for IntroArg rules, clean up proofs
- GaloisInc/saw-core@fcb8625 more tweaks to proof automation
- GaloisInc/saw-core@7ac5115 move bv hints to SAWCoreBitvectors
- GaloisInc/saw-core@59bc79a performance improvements to prove_refinement...
- GaloisInc/saw-core@1fa5049 add `refines` and basic properties, more clean up, some partial progress
- GaloisInc/saw-core@f0ed599 Adds bvShl and enables CryptolPrimitivesForSAWCore to build

saw-core-coq/src/Verifier/SAW/Translation/Coq/SpecialTreatment.hs
@@ -266,9 +266,6 @@ sawCorePreludeSpecialTreatmentMap configuration =
   [ ("Eq",      mapsTo sawDefinitionsModule "Eq")
   , ("Eq__rec", mapsTo sawDefinitionsModule "Eq__rec")
   , ("Refl",    mapsTo sawDefinitionsModule "Refl")
-  , ("EqP",      mapsTo sawDefinitionsModule "EqP")
-  , ("EqP__rec", mapsTo sawDefinitionsModule "EqP__rec")
-  , ("ReflP",    mapsTo sawDefinitionsModule "ReflP")
   ]
 
   -- Strings
@@ -444,12 +441,6 @@ sawCorePreludeSpecialTreatmentMap configuration =
   , ("Nil", replace (Coq.ExplVar "Datatypes.nil"))
   , ("Cons", replace (Coq.ExplVar "Datatypes.cons"))
   , ("List__rec", replace (Coq.ExplVar "Datatypes.list_rect"))
-  ]
-
-  -- Definitions that depend on axioms currently skipped
-  ++
-  [ ("composeM",   skip)
-  , ("letRecFuns", skip)
   ]
 
 constantsRenamingMap :: [(String, String)] -> Map.Map String String
