saw-core-coq/coq/handwritten/CryptolToCoq/SAWCorePreludeExtra.v
@@ -1,4 +1,5 @@
 From Coq          Require Import Lists.List.
+From Coq          Require Import Logic.FunctionalExtensionality.
 Import ListNotations.
 From Coq          Require Import String.
 From Coq          Require Import Vectors.Vector.
@@ -58,4 +59,22 @@ Proof.
     simpl.
     intuition.
   }
+Qed.
+
+Theorem fold_unfold_IRT As Ds D : forall x, foldIRT As Ds D (unfoldIRT As Ds D x) = x.
+Proof.
+  induction x; simpl; unfold uncurry; f_equal; try easy.
+  (* All that remains is the IRT_BVVec case, which requires functional extensionality
+     and the fact that genBVVec and atBVVec define an isomorphism *)
+  repeat (apply functional_extensionality_dep; intro).
+  rewrite at_gen_BVVec; eauto.
+Qed.
+
+Theorem unfold_fold_IRT As Ds D : forall u, unfoldIRT As Ds D (foldIRT As Ds D u) = u.
+Proof.
+  revert Ds; induction D; try destruct u; simpl; f_equal; try easy.
+  (* All that remains is the IRT_BVVec case, which requires functional extensionality
+     and the fact that genBVVec and atBVVec define an isomorphism *)
+  intros; rewrite <- (gen_at_BVVec _ _ _ u).
+  f_equal; repeat (apply functional_extensionality_dep; intro); eauto.
 Qed.
